Finish the proofs in Hacl.Streaming.Blake2s_32.fst

code/streaming/Hacl.Streaming.Blake2s_32.fst
@@ -37,8 +37,6 @@ open Hacl.Impl.Blake2.Generic
 module Impl = Hacl.Impl.Blake2.Generic
 module Incr = Spec.Hash.Incremental
 
-//open Hacl.Blake2s_32
-
 /// An instance of the stateful type class for blake2
 /// =========================================================
 
@@ -57,41 +55,32 @@ let to_hash_alg (a : Spec.alg) =
 
 let index = unit
 
-/// The stateful state: (wv, hash, *total_len)
-/// The total_len pointer should actually be ghost
+/// The stateful state: (wv, hash)
 inline_for_extraction noextract
-let s = state_p a m & state_p a m & B.pointer (Hash.extra_state (to_hash_alg a))
+let s = state_p a m & state_p a m
 
 inline_for_extraction noextract
 let extra_state_zero_element a : Hash.extra_state (to_hash_alg a) =
   Hash.nat_to_extra_state (to_hash_alg a) 0
 
 inline_for_extraction noextract
-let t = Hash.words_state (to_hash_alg a)
+let t = Hash.words_state' (to_hash_alg a)
 
 inline_for_extraction noextract
 let get_wv (s : s) : Tot (state_p a m) =
-  match s with wv, _, _ -> wv
+  match s with wv, _ -> wv
 
 inline_for_extraction noextract
 let get_state_p (s : s) : Tot (state_p a m) =
-  match s with _, p, _ -> p
+  match s with _, p -> p
 
 inline_for_extraction noextract
 let state_v (h : HS.mem) (s : s) : GTot (Spec.state a) =
   Core.state_v h (get_state_p s)
 
 inline_for_extraction noextract
-let get_extra_state_p (s : s) : Tot (B.pointer (Hash.extra_state (to_hash_alg a))) =
-  match s with _, _, l -> l
-
-(*inline_for_extraction noextract
-let extra_state_v (h : HS.mem) (s : s) : GTot (Hash.extra_state (to_hash_alg a))=
-  B.deref h (get_extra_state_p s) *)
-
-inline_for_extraction noextract
 let s_v (h : HS.mem) (s : s) : GTot t =
-  state_v h s, B.deref h (get_extra_state_p s) //extra_state_v h s
+  state_v h s
 
 /// Small helper which facilitates inferencing implicit arguments for buffer
 /// operations
@@ -106,57 +95,49 @@ let stateful_blake2s_32: I.stateful unit =
     (fun () -> s) (* s *)
     (* footprint *)
     (fun #_ _ acc ->
-      let wv, b, l = acc in
+      let wv, b = acc in
       B.loc_union
-        (B.loc_union
-          (B.loc_addr_of_buffer (state_to_lbuffer wv))
-          (B.loc_addr_of_buffer (state_to_lbuffer b)))
-        (B.loc_addr_of_buffer l))
+       (B.loc_addr_of_buffer (state_to_lbuffer wv))
+       (B.loc_addr_of_buffer (state_to_lbuffer b)))
     (* freeable *)
     (fun #_ _ acc ->
-      let wv, b, l = acc in
+      let wv, b = acc in
       B.freeable (state_to_lbuffer wv) /\
-      B.freeable (state_to_lbuffer b) /\
-      B.freeable l)
+      B.freeable (state_to_lbuffer b))
     (* invariant *)
     (fun #_ h acc ->
-      let wv, b, l = acc in
+      let wv, b = acc in
       B.live h (state_to_lbuffer wv) /\
       B.live h (state_to_lbuffer b) /\
-      B.live h l /\
-      B.disjoint (state_to_lbuffer wv) (state_to_lbuffer b) /\
-      B.disjoint (state_to_lbuffer wv) l /\
-      B.disjoint (state_to_lbuffer b) l)
+      B.disjoint (state_to_lbuffer wv) (state_to_lbuffer b))
     (fun () -> t) (* t *)
     (fun () h acc -> s_v h acc) (* v *)
-    (fun #_ h acc -> let wv, b, l = acc in ()) (* invariant_loc_in_footprint *)
-    (fun #_ l acc h0 h1 -> let wv, b, l = acc in ()) (* frame_invariant *)
+    (fun #_ h acc -> let wv, b = acc in ()) (* invariant_loc_in_footprint *)
+    (fun #_ l acc h0 h1 -> let wv, b = acc in ()) (* frame_invariant *)
     (fun #_ _ _ _ _ -> ()) (* frame_freeable *)
     (* alloca *)
     (fun () ->
       let wv = alloc_state a m in
       let b = alloc_state a m in
-      let l = B.alloca (extra_state_zero_element a) (U32.uint_to_t 1) in
-      wv, b, l)
+//      let l = B.alloca (extra_state_zero_element a) (U32.uint_to_t 1) in
+      wv, b)
     (* create_in *)
     (fun () r ->
       let wv = B.malloc r (zero_element a m) U32.(4ul *^ row_len a m) in
       let b = B.malloc r (zero_element a m) U32.(4ul *^ row_len a m) in
-      let l = B.malloc r (extra_state_zero_element a) (U32.uint_to_t 1) in
-      wv, b, l)
+//      let l = B.malloc r (extra_state_zero_element a) (U32.uint_to_t 1) in
+      wv, b)
     (* free *)
     (fun _ acc ->
-      match acc with wv, b, l ->
+      match acc with wv, b ->
       B.free (state_to_lbuffer wv);
-      B.free (state_to_lbuffer b);
-      B.free l)
+      B.free (state_to_lbuffer b))
     (* copy *)
     (fun _ src dst ->
-      match src with src_wv, src_b, src_l ->
-      match dst with src_wv, dst_b, dst_l ->
+      match src with src_wv, src_b ->
+      match dst with src_wv, dst_b ->
       B.blit (state_to_lbuffer src_b) 0ul (state_to_lbuffer dst_b) 0ul
-             U32.(4ul *^ row_len a m);
-      B.blit src_l 0ul dst_l 0ul 1ul)
+             U32.(4ul *^ row_len a m))
 
 inline_for_extraction noextract
 let k (key_size : nat{0 < key_size /\ key_size <= Spec.max_key a}) =
@@ -184,14 +165,57 @@ let output_size : nat = Spec.max_output a
 inline_for_extraction noextract
 let output_len = U32.uint_to_t output_size
 
-let init_s () key : Hash.words_state (to_hash_alg a) =
-  Spec.blake2_init a key_size key output_size,
-  Hash.nat_to_extra_state (to_hash_alg a) (Spec.compute_prev0 a key_size)
-  //extra_state_zero_element a
-let update_s () acc = Agile.update (to_hash_alg a)
-let update_multi_s () = Agile.update_multi (to_hash_alg a)
-let update_last_s () = Spec.Hash.Incremental.update_last (to_hash_alg a)
-let finish_s () = Spec.Hash.PadFinish.finish (to_hash_alg a)
+/// The prevlen parameter computed by the streaming functor and given to ``update_multi``
+/// or ``update_last`` is equal to the length of the data processed so far (without the
+/// key). In the case of blake2, however, we also need to count the key (if it is not
+/// an empty seq) in the total length of processed data.
+inline_for_extraction noextract
+let blake2_prevlen_nat (key_size : nat) (prevlen : nat) : nat =
+  if key_size = 0 then prevlen else prevlen + Spec.size_block a
+
+/// Same function as above but with low-level types
+inline_for_extraction noextract
+let blake2_prevlen_ (key_size : nat)
+                    (prevlen : U64.t{ U64.v prevlen <= max_input_length key_size }) :
+  x:U64.t { U64.v x = blake2_prevlen_nat key_size (U64.v prevlen) } =
+  if key_size = 0 then prevlen
+  else U64.(prevlen +^ FStar.Int.Cast.uint32_to_uint64 block_len)
+
+inline_for_extraction noextract
+let blake2_prevlen (key_size : nat)
+                   (prevlen : U64.t{ U64.v prevlen <= max_input_length key_size }) :
+  x:Spec.limb_t a {
+    Lib.IntTypes.uint_v x = blake2_prevlen_nat key_size (U64.v prevlen) } =
+  let open Lib.IntTypes in
+  match a with
+  | Spec.Blake2S -> to_u64 #U64 #PUB (blake2_prevlen_ key_size prevlen)
+  | Spec.Blake2B -> FStar.Int.Cast.Full.uint64_to_uint128
+                     (to_u64 #U64 #PUB (blake2_prevlen_ key_size prevlen))
+
+let init_s () (key : Seq.lseq uint8 key_size) : Tot t =
+  Spec.blake2_init a key_size key output_size
+
+let update_multi_s () (acc : t) (prevlen : nat{prevlen % Spec.size_block a = 0})
+                   (input : Seq.seq uint8{ prevlen + S.length input <= max_input_length key_size /\
+                                           S.length input % Spec.size_block a = 0 }) :
+  Tot t =
+  let es = Hash.nat_to_extra_state (to_hash_alg a) (blake2_prevlen_nat key_size prevlen) in
+  let s = (acc, es) in
+  fst (Agile.update_multi (to_hash_alg a) s input)
+
+let update_last_s () (acc : t) (prevlen : nat{prevlen % Spec.size_block a = 0})
+                  (input : Seq.seq uint8{ S.length input + prevlen <= max_input_length key_size /\
+                                          S.length input <= Spec.size_block a }) :
+  Tot t =
+  let es = Hash.nat_to_extra_state (to_hash_alg a) (blake2_prevlen_nat key_size prevlen) in
+  let s = (acc, es) in
+  fst (Spec.Hash.Incremental.update_last (to_hash_alg a) s prevlen input)
+
+let finish_s () (key : Seq.lseq uint8 key_size) (acc : t) :
+  output : S.seq uint8 { S.length output = U32.v output_len } =
+  (* The extra state is actually not used, so we initialize it to a dummy value *)
+  let s = (acc, Hash.nat_to_extra_state (to_hash_alg a) 0) in
+  Spec.Hash.PadFinish.finish (to_hash_alg a) s
 
 let spec_s ()
            (key : S.seq uint8{S.length key = key_size})
@@ -203,91 +227,165 @@ let spec_s ()
 val update_multi_zero:
   i:index ->
   acc:t ->
+  prevlen:nat{prevlen % Spec.size_block a = 0} ->
   Lemma
-  (ensures (update_multi_s i acc S.empty == acc))
+  (requires (prevlen <= max_input_length key_size))
+  (ensures (update_multi_s i acc prevlen S.empty == acc))
 
-let update_multi_zero () acc =
-  Spec.Hash.Lemmas.update_multi_zero (to_hash_alg a) acc
+let update_multi_zero () acc prevlen =
+  let es = Hash.nat_to_extra_state (to_hash_alg a) (blake2_prevlen_nat key_size prevlen) in
+  let s = (acc, es) in
+  Spec.Hash.Lemmas.update_multi_zero (to_hash_alg a) s
 
-val  update_multi_associative:
+val update_multi_associative:
   i:index ->
   acc: t ->
+  prevlen1:nat ->
+  prevlen2:nat ->
   input1:S.seq uint8 ->
   input2:S.seq uint8 ->
   Lemma
   (requires (
-    S.length input1 % U32.v block_len = 0 /\
-    S.length input2 % U32.v block_len = 0))
+    prevlen1 % Spec.size_block a = 0 /\
+    S.length input1 % Spec.size_block a = 0 /\
+    S.length input2 % Spec.size_block a = 0 /\
+    prevlen1 + S.length input1 + S.length input2 <= max_input_length key_size /\
+    prevlen2 = prevlen1 + S.length input1))
   (ensures (
     let input = S.append input1 input2 in
-    S.length input % U32.v block_len = 0 /\
-    update_multi_s i (update_multi_s i acc input1) input2 ==
-      update_multi_s i acc input))
+    S.length input % Spec.size_block a = 0 /\
+    prevlen2 % Spec.size_block a = 0 /\
+    update_multi_s i (update_multi_s i acc prevlen1 input1) prevlen2 input2 ==
+      update_multi_s i acc prevlen1 input))
 
-let update_multi_associative () acc input1 input2 =
-  Spec.Hash.Lemmas.update_multi_associative (to_hash_alg a) acc input1 input2
+let update_multi_associative () acc prevlen1 prevlen2 input1 input2 =
+  let es = Hash.nat_to_extra_state (to_hash_alg a) (blake2_prevlen_nat key_size prevlen1) in
+  let s = (acc, es) in
+  Spec.Hash.Lemmas.update_multi_associative (to_hash_alg a) s input1 input2;
+  Spec.Hash.Incremental.Lemmas.update_multi_extra_state_eq (to_hash_alg a) s input1;
+  Spec.Hash.Lemmas.extra_state_add_nat_bound_lem2 #(to_hash_alg a) es (S.length input1)
+ 
+/// A helper function: the hash incremental function defined with the functions
+/// locally defined (with a signature adapted to the functor).
+val blake2_hash_incremental_s :
+  i:index ->
+  key: I.((k key_size).t ()) ->
+  input:S.seq uint8 { S.length input <= max_input_length key_size } ->
+  output:S.seq uint8 { S.length output = output_size }
 
+let blake2_hash_incremental_s i key input =
+  let bs, l = Spec.Hash.Incremental.split_blocks (to_hash_alg a) input in
+  let acc1 = init_s i key in
+  let acc2 = update_multi_s i acc1 0 bs in
+  let acc3 = update_last_s i acc2 (S.length bs) l in
+  let acc4 = finish_s i key acc3 in
+  acc4
+
+/// This helper lemma proves that the blake2 specification functions defined above
+/// with a signature adapted to the functor give the same result, if properly called,
+/// as the original hash incremental functions.
+val blake2_hash_incremental_s_is_hash_incremental :
+  i:index ->
+  key: I.((k key_size).t ()) ->
+  input:S.seq uint8 { S.length input <= max_input_length key_size } ->
+  Lemma(
+    blake2_hash_incremental_s i key input ==
+      Spec.Hash.Incremental.blake2_hash_incremental (to_hash_alg a) key_size key input)
+
+/// TODO: make the proof stable
+let blake2_hash_incremental_s_is_hash_incremental i key input =
+  let bs, l = Spec.Hash.Incremental.split_blocks (to_hash_alg a) input in
+  let acc1 = init_s i key in
+  let acc2 = update_multi_s i acc1 0 bs in
+  let acc3 = update_last_s i acc2 (S.length bs) l in
+  let acc4 = finish_s i key acc3 in
+  assert(acc4 == blake2_hash_incremental_s i key input); (* sanity check *)
+  let s1 = Spec.Hash.Incremental.blake2_init (to_hash_alg a) key_size key in
+  let s2 = Agile.update_multi (to_hash_alg a) s1 bs in
+  let prevlen = S.length bs in (* dummy value: this variable is actually not used *)
+  let s3 = Spec.Hash.Incremental.update_last (to_hash_alg a) s2 prevlen l in
+  let s4 = Spec.Hash.PadFinish.finish (to_hash_alg a) s3 in
+  let s4' = Spec.Hash.Incremental.blake2_hash_incremental (to_hash_alg a) key_size key input in
+  assert(s4 == s4'); (* sanity check *)
+  (* The proof *)
+  let es1 = Hash.nat_to_extra_state (to_hash_alg a) (blake2_prevlen_nat key_size 0) in
+  let s1' = (acc1, es1) in
+  assert(s1' == s1);
+  Spec.Hash.Incremental.Lemmas.update_multi_extra_state_eq (to_hash_alg a) s1 bs;
+  Spec.Hash.Lemmas.extra_state_add_nat_bound_lem2 #(to_hash_alg a) es1 (S.length bs);
+  let es2 = Hash.nat_to_extra_state (to_hash_alg a) (blake2_prevlen_nat key_size (S.length bs)) in
+  let s2' = (acc2, es2) in
+  assert(s2' == s2);
+  let es3 = Hash.nat_to_extra_state (to_hash_alg a) 0 in
+  let s3' = (acc3, es3) in
+  assert(s3' == s3);
+  assert(acc4 == s4)
+
+/// TODO: make stable
 val spec_is_incremental:
   i:index ->
   key: I.((k key_size).t ()) ->
   input:S.seq uint8 { S.length input <= max_input_length key_size } ->
-  Lemma (ensures (
-    let open FStar.Mul in
-    let block_length = U32.v block_len in
-    let n = S.length input / block_length in
-    let rem = S.length input % block_length in
-    let n, rem = if rem = 0 && n > 0 then n - 1, block_length else n, rem in
-    let bs, l = S.split input (n * block_length) in
-    (**) FStar.Math.Lemmas.multiple_modulo_lemma n block_length;
-    let hash = update_multi_s i (init_s i key) bs in
-    let hash = update_last_s i hash (n * block_length) l in
-    finish_s i hash `S.equal` spec_s i key input))
+  Lemma (
+    let bs, l = Spec.Hash.Incremental.split_blocks (to_hash_alg a) input in
+    let hash = update_multi_s i (init_s i key) 0 bs in
+    let hash = update_last_s i hash (S.length bs) l in
+    finish_s i key hash `S.equal` spec_s i key input)
 
-let spec_is_incremental () key input =
+let spec_is_incremental i key input =
+  blake2_hash_incremental_s_is_hash_incremental i key input;
   Spec.Hash.Incremental.blake2_is_hash_incremental (to_hash_alg a) key_size key input
 
 val update_multi_eq :
   nb : nat ->
+  acc : t ->
+  prevlen : nat {prevlen % Spec.size_block a = 0 } ->
   blocks : S.seq uint8 ->
-  acc : Hash.words_state (to_hash_alg a) ->
   Lemma
     (requires (
-      Hash.extra_state_v (snd acc) + S.length blocks <= Spec.max_limb a /\
-      Hash.extra_state_v (snd acc) + S.length blocks <= Hash.max_extra_state (to_hash_alg a) /\
+      prevlen + S.length blocks <= max_input_length key_size /\
+      blake2_prevlen_nat key_size prevlen + S.length blocks <= Hash.max_extra_state (to_hash_alg a) /\
       S.length blocks = Hash.block_length (to_hash_alg a) * nb))
     (ensures (
-      let prev_length = Hash.extra_state_v (snd acc) in
-      (Loops.repeati #(Hash.words_state' (to_hash_alg a)) nb (Spec.blake2_update1 a prev_length blocks) (fst acc),
-       Hash.extra_state_add_nat #(to_hash_alg a) (snd acc) (S.length blocks)) ==
-       update_multi_s () acc blocks))
+      let prevlen' = blake2_prevlen_nat key_size prevlen in
+      update_multi_s () acc prevlen blocks ==
+        Loops.repeati #(Hash.words_state' (to_hash_alg a)) nb
+                       (Spec.blake2_update1 a prevlen' blocks) acc))
 
-let update_multi_eq nb blocks acc =
+let update_multi_eq nb acc prevlen blocks =
   let blocks', _ = Seq.split blocks (nb * Hash.block_length (to_hash_alg a)) in
   assert(blocks' `Seq.equal` blocks);
-  let prev_length = Hash.extra_state_v (snd acc) in
+  let prevlen' = blake2_prevlen_nat key_size prevlen in
+  let es = Hash.nat_to_extra_state (to_hash_alg a) prevlen' in
   Spec.Hash.Incremental.repeati_blake2_update1_is_update_multi (to_hash_alg a)
-                                                               nb prev_length
-                                                               blocks (fst acc);
-  Spec.Hash.Lemmas.extra_state_add_nat_bound_lem1 #(to_hash_alg a) (snd acc) (S.length blocks);
+                                                               nb prevlen'
+                                                               blocks acc;
+  Spec.Hash.Lemmas.extra_state_add_nat_bound_lem1 #(to_hash_alg a) es (S.length blocks);
   assert(
-    Hash.nat_to_extra_state (to_hash_alg a) (prev_length + S.length blocks) ==
-    Hash.extra_state_add_nat #(to_hash_alg a) (snd acc) (S.length blocks))
+    Hash.nat_to_extra_state (to_hash_alg a) (prevlen' + S.length blocks) ==
+    Hash.extra_state_add_nat #(to_hash_alg a) es (S.length blocks))
 
 val update_last_eq :
-  prev_length : nat{prev_length % Hash.block_length (to_hash_alg a) = 0} ->
+  prevlen : nat{prevlen % Hash.block_length (to_hash_alg a) = 0} ->
   last : S.seq uint8 {S.length last <= Hash.block_length (to_hash_alg a) /\
-                      prev_length + S.length last <= max_input_length key_size} ->
-  acc : Hash.words_state (to_hash_alg a) ->
+                      prevlen + S.length last <= max_input_length key_size} ->
+  acc : t ->
   Lemma
-  (requires (prev_length = Hash.extra_state_v #(to_hash_alg a) (snd acc)))
   (ensures (
-    Spec.blake2_update_last a prev_length (S.length last) last (fst acc) ==
-      fst (update_last_s () acc prev_length last)))
+    let prevlen' = blake2_prevlen_nat key_size prevlen in
+    Spec.blake2_update_last a prevlen' (S.length last) last acc ==
+      update_last_s () acc prevlen last))
 
-let update_last_eq prev_length last acc =
+/// TODO: make stable
+let update_last_eq prevlen last acc =
   (* Checking how to unfold the ``update_last_s`` definition *)
-  let accf = update_last_s () acc prev_length last in
-  assert(accf == Spec.Hash.Incremental.update_last_blake (to_hash_alg a) acc prev_length last);
+  let prevlen' = blake2_prevlen_nat key_size prevlen in
+  let es = Hash.nat_to_extra_state (to_hash_alg a) prevlen' in
+  let s = acc, es in
+  let s' = Spec.Hash.Incremental.update_last_blake (to_hash_alg a) s prevlen' last in
+  (* TODO: if accf is defined before s', the proof loops at the definition of s' *)
+  let accf = update_last_s () acc prevlen last in
+  assert(accf == fst s');
   (* Make sure the blocks decomposition is what we expect *)
   let blocks, last_block, rem = Spec.Hash.Incremental.last_split_blake (to_hash_alg a) last in
   assert(blocks `S.equal` S.empty);
@@ -295,13 +393,13 @@ let update_last_eq prev_length last acc =
   assert(last_block == Spec.get_last_padded_block a last (S.length last));
   (* Prove that the last call to ``update_multi`` does nothing (there is no call to
    * ``update_multi`` in ``blake2_update_last`` *)
-  let acc2 = Spec.Agile.Hash.update_multi (to_hash_alg a) acc blocks in
-  Spec.Hash.Lemmas.update_multi_zero (to_hash_alg a) acc;
-  assert(acc2 == acc);
+  let s2 = Spec.Agile.Hash.update_multi (to_hash_alg a) s blocks in
+  Spec.Hash.Lemmas.update_multi_zero (to_hash_alg a) s;
+  assert(s2 == s);
   (* Prove that the extra state update computes the same total length as in ``blake2_update_last`` *)
-  Spec.Hash.Lemmas.extra_state_add_nat_bound_lem1 #(to_hash_alg a) (snd acc) (S.length last);
-  assert(Hash.extra_state_v (Hash.extra_state_add_nat (snd acc) (S.length last)) ==
-         Hash.extra_state_v (snd acc) + S.length last)
+  Spec.Hash.Lemmas.extra_state_add_nat_bound_lem1 #(to_hash_alg a) es (S.length last);
+  assert(Hash.extra_state_v (Hash.extra_state_add_nat es (S.length last)) ==
+         Hash.extra_state_v es + S.length last)
 
 /// Equality between the state types defined by blake2s and the generic hash.
 /// The equality is not trivial because of subtleties linked to the way types are
@@ -317,9 +415,99 @@ let state_types_equalities () =
   assert_norm(lseq (Spec.row a) 4 == m:Seq.seq (Spec.row a) {Seq.length m == 4});
   assert(lseq (Spec.row a) 4 == m:Seq.seq (Spec.row a) {Seq.length m = 4})
 
-#push-options "--z3rlimit 500 --ifuel 1 --print_implicits"
+(* TODO: find a way not to duplicate the block spec *)
+val update_multi: (i:G.erased index -> (
+  let i = G.reveal i in
+  s:s ->
+  prevlen:U64.t { U64.v prevlen % U32.v (block_len) = 0 } ->
+  blocks:B.buffer uint8 { B.length blocks % U32.v (block_len) = 0 } ->
+  len: U32.t { U32.v len = B.length blocks /\
+               U64.v prevlen + U32.v len <= max_input_length key_size } ->
+  ST.Stack unit
+  (requires fun h0 ->
+    let state = stateful_blake2s_32 in
+    state.I.invariant #i h0 s /\
+    B.live h0 blocks /\
+    B.(loc_disjoint (state.I.footprint #i h0 s) (loc_buffer blocks)))
+  (ensures fun h0 _ h1 ->
+    let state = stateful_blake2s_32 in
+    B.(modifies (state.I.footprint #i h0 s) h0 h1) /\
+    state.I.footprint #i h0 s == state.I.footprint #i h1 s /\
+    state.I.invariant #i h1 s /\
+    state.I.v i h1 s == update_multi_s i (state.I.v i h0 s) (U64.v prevlen) (B.as_seq h0 blocks) /\
+    (state.I.freeable #i h0 s ==> state.I.freeable #i h1 s))))
+
+let update_multi i acc prevlen blocks len =
+  [@inline_let] let wv = get_wv acc in
+  [@inline_let] let h = get_state_p acc in
+  (**) let h0 = ST.get () in
+  let nb = U32.(len /^ block_len) in
+  [@inline_let] let prevlen' = blake2_prevlen key_size prevlen in
+  Impl.blake2_update_multi #a #m #len (Impl.blake2_update_block #a #m) wv h
+                           prevlen' blocks nb;
+  (**) let h3 = ST.get () in
+  (**) assert(s_v h3 acc ==
+  (**)    Loops.repeati #(Spec.Blake2.state a) (U32.v nb)
+  (**)                  (Spec.blake2_update1 a (Lib.IntTypes.uint_v prevlen')
+  (**)                                       (B.as_seq h0 blocks))
+  (**)                  (s_v h0 acc));
+  (**) state_types_equalities ();
+  (**) assert(Spec.Blake2.state a == Hash.words_state' (to_hash_alg a));
+  (**) update_multi_eq (U32.v nb) (s_v h0 acc) (U64.v prevlen) (B.as_seq h0 blocks);
+  (**) assert(Lib.IntTypes.uint_v prevlen' = blake2_prevlen_nat key_size (U64.v prevlen));
+  (**) assert(s_v h3 acc == update_multi_s () (s_v h0 acc) (U64.v prevlen) (B.as_seq h0 blocks));
+  (**) assert(B.(modifies (stateful_blake2s_32.I.footprint #() h0 acc) h0 h3))
+
+val update_last: (
+  i: G.erased index -> (
+  let i = G.reveal i in
+  s:s ->
+  prevlen:U64.t { U64.v prevlen % U32.v (block_len) = 0 } ->
+  last:B.buffer uint8 ->
+  last_len:U32.t{
+    last_len = B.len last /\
+    U32.v last_len <= U32.v (block_len) /\
+    U64.v prevlen + U32.v last_len <= max_input_length key_size} ->
+  ST.Stack unit
+  (requires fun h0 ->
+    let state = stateful_blake2s_32 in
+    state.I.invariant #i h0 s /\
+    B.live h0 last /\
+    B.(loc_disjoint (state.I.footprint #i h0 s) (loc_buffer last)))
+  (ensures fun h0 _ h1 ->
+    let state = stateful_blake2s_32 in
+    state.I.invariant #i h1 s /\
+    state.I.v i h1 s == update_last_s i (state.I.v i h0 s) (U64.v prevlen) (B.as_seq h0 last) /\
+    B.(modifies (state.I.footprint #i h0 s) h0 h1) /\
+    state.I.footprint #i h0 s == state.I.footprint #i h1 s /\
+    (state.I.freeable #i h0 s ==> state.I.freeable #i h1 s))))
+
+let update_last _ acc prevlen last last_len =
+  [@inline_let] let wv = get_wv acc in
+  [@inline_let] let h = get_state_p acc in
+  (**) let h0 = ST.get () in
+  (**) assert_norm(U64.v prevlen + U32.v last_len <= Spec.Blake2.max_limb a);
+  [@inline_let]
+  let prevlen' = blake2_prevlen key_size prevlen in
+  assert((U64.v prevlen) % Hash.block_length (to_hash_alg a) = 0);
+  assert(B.length last <= Hash.block_length (to_hash_alg a));
+  assert(U64.v prevlen + B.length last <= max_input_length key_size);
+  (* TODO: this call loops if moved at the end of the proof *)
+  (**) update_last_eq (U64.v prevlen) (B.as_seq h0 last) (s_v h0 acc);
+  Impl.blake2_update_last #a #m (Impl.blake2_update_block #a #m) #last_len
+                          wv h prevlen' last_len last;
+  (**) let h2 = ST.get () in
+  (**) assert(
+  (**)   Core.state_v h2 h ==
+  (**)     Spec.blake2_update_last a (Lib.IntTypes.uint_v prevlen') (U32.v last_len)
+  (**)                               (B.as_seq h0 last)
+  (**)                               (Core.state_v h0 h));
+  (**) assert(s_v h2 acc ==
+  (**)   update_last_s () (s_v h0 acc) (U64.v prevlen) (B.as_seq h0 last))
+
+#push-options "--ifuel 1"
 inline_for_extraction noextract
-let blake2s_32 : I.block unit =
+let blake2s_32 (* : I.block unit *) =
   I.Block
     I.Erased (* key management *)
     
@@ -331,13 +519,15 @@ let blake2s_32 : I.block unit =
     (fun () -> block_len) (* block_len *)
     
     (fun () k -> init_s () k) (* init_s *)
-    (fun () acc input -> update_multi_s () acc input) (* update_multi_s *)
+    (fun () acc prevlen input -> update_multi_s () acc prevlen input) (* update_multi_s *)
     (fun () acc prevlen input -> update_last_s () acc prevlen input) (* update_last_s *)
-    (fun () k acc -> finish_s () acc) (* finish_s *)
+    (fun () k acc -> finish_s () k acc) (* finish_s *)
     (fun () -> spec_s ()) (* spec_s *)
 
-    (fun () acc -> update_multi_zero () acc) (* update_multi_zero *)
-    (fun () acc input1 input2 -> update_multi_associative () acc input1 input2) (* update_multi_associative *)
+    (fun () prevlen acc -> update_multi_zero () prevlen acc) (* update_multi_zero *)
+    (* update_multi_associative *)
+    (fun () acc prevlen1 prevlen2 input1 input2 ->
+      update_multi_associative () acc prevlen1 prevlen2 input1 input2)
     (fun () k input -> spec_is_incremental () k input) (* spec_is_incremental *)
     (fun _ acc -> ()) (* index_of_state *)
 
@@ -345,70 +535,14 @@ let blake2s_32 : I.block unit =
     (fun _ key acc ->
       [@inline_let] let wv = get_wv acc in
       [@inline_let] let h = get_state_p acc in
-      [@inline_let] let es = get_extra_state_p acc in
-      Impl.blake2_init #a #m (Impl.blake2_update_block #a #m) wv h key_len key output_len;
-      B.upd es 0ul (Hash.nat_to_extra_state (to_hash_alg a) (Spec.compute_prev0 a key_size)))
+      Impl.blake2_init #a #m (Impl.blake2_update_block #a #m) wv h key_len key output_len)
 
     (* update_multi *)
-    (fun _ acc blocks len ->
-      [@inline_let] let wv = get_wv acc in
-      [@inline_let] let h = get_state_p acc in
-      [@inline_let] let es = get_extra_state_p acc in
-      (**) let h0 = ST.get () in
-      let prev = B.index es 0ul in
-      (* TODO: add the following assumption to the signature? *)
-      (**) assume(Hash.extra_state_v prev + U32.v len <= max_input_length key_size);
-      let nb = U32.(len /^ block_len) in
-      Impl.blake2_update_multi #a #m #len (Impl.blake2_update_block #a #m) wv h prev blocks nb;
-      [@inline_let] let totlen = Hash.extra_state_add_size_t #(to_hash_alg a) prev len in
-      B.upd es 0ul totlen;
-      (**) let h3 = ST.get () in
-      (**) assert(fst (s_v h3 acc) ==
-      (**)    Loops.repeati #(Spec.Blake2.state a) (U32.v nb)
-      (**)                  (Spec.blake2_update1 a (Hash.extra_state_v prev)
-      (**)                  (B.as_seq h0 blocks))
-      (**)                  (fst (s_v h0 acc)));
-      (**) state_types_equalities ();
-      (**) assert(Spec.Blake2.state a == Hash.words_state' (to_hash_alg a));
-      (**) update_multi_eq (U32.v nb) (B.as_seq h0 blocks) (s_v h0 acc);
-      (**) assert(s_v h3 acc == update_multi_s () (s_v h0 acc) (B.as_seq h0 blocks));
-      (**) assert(B.(modifies (stateful_blake2s_32.I.footprint #() h0 acc) h0 h3)))
+    (fun _ acc prevlen blocks len -> update_multi () acc prevlen blocks len)
 
     (* update_last *)
-    (fun _ acc prev_len last last_len ->
-      (* TODO: use the extra state and not prev_len - they are not the same *)
-      [@inline_let] let wv = get_wv acc in
-      [@inline_let] let h = get_state_p acc in
-      [@inline_let] let es = get_extra_state_p acc in
-      (**) let h0 = ST.get () in
-      (**) assert_norm(U64.v prev_len + U32.v last_len <= Spec.Blake2.max_limb a);
-      [@inline_let]
-      let prev_len' : Spec.Blake2.limb_t a =
-        match a with
-        | Spec.Blake2S -> Lib.IntTypes.(cast #U64 #PUB U64 SEC prev_len)
-        | Spec.Blake2B -> FStar.Int.Cast.Full.uint64_to_uint128 prev_len
-      in
-      Impl.blake2_update_last #a #m (Impl.blake2_update_block #a #m) #last_len
-                              wv h prev_len' last_len last;
-      B.upd es 0ul (extra_state_zero_element a);
-      (**) let h2 = ST.get () in
-      (**) assert(
-      (**)   Core.state_v h2 h ==
-      (**)     Spec.blake2_update_last a (U64.v prev_len) (U32.v last_len) (B.as_seq h0 last)
-      (**)                               (Core.state_v h0 h));
-      (* TODO: I think we could remove the extra state from the concrete implementation
-       * of ``words_state`` and add a ``prev_len`` parameter wherever necessary.
-       * Update: actually, it will cause problem because of the [init]. We need to
-       * ignore the prevlen parameter in the interface and always use the extra state,
-       * which can't be ghost. But this will cause problem in update_multi...
-       * To solve the init problem: we could add size_block to prevlen by checking the size
-       * of the key (and this check could be normalized at extraction) and remove the extra
-       * state. *)
-      (**) assume(U64.v prev_len = Hash.extra_state_v (snd (s_v h0 acc)));
-      (**) update_last_eq (U64.v prev_len) (B.as_seq h0 last) (s_v h0 acc);
-      (**) assert(s_v h2 acc ==
-      (**)   update_last_s () (s_v h0 acc) (U64.v prev_len) (B.as_seq h0 last))
-      )
+    (fun _ acc prevlen last last_len ->
+      update_last () acc prevlen last last_len)
 
     (* finish *)
     (fun _ k acc dst ->
